theories/SLOT/Generator.v
@@ -1,0 +1,95 @@
+(** * Lazy definition of Ensemble
+ *)
+
+From Coq Require Import
+     Program.Basics
+     List.
+
+Import ListNotations.
+
+From LibTx Require Import
+     Misc
+     EventTrace
+     Permutation
+     SLOT.Hoare
+     SLOT.Ensemble.
+
+Section defn.
+  Context `{Hssp : StateSpace}.
+
+  Class Generator (A : Type) :=
+    { next : A -> option (TE * A) -> Prop
+    }.
+
+  Section unfold.
+    Context {G} `{Generator G}.
+
+    Inductive UnfoldsTo (g : G) : list TE -> Prop :=
+    | gen_unf_nil :
+        (next g) None ->
+        UnfoldsTo g []
+    | gen_unf_cons : forall te g' l,
+        (next g) (Some (te, g')) ->
+        UnfoldsTo g' l ->
+        UnfoldsTo g (te :: l).
+  End unfold.
+
+  Global Instance listGenerator : Generator (list TE) :=
+    {| next l :=
+         match l with
+         | [] => eq None
+         | a :: l => eq (Some (a, l))
+         end
+    |}.
+
+  Lemma unfold_list_generator : forall (l l' : list TE),
+      UnfoldsTo l l' ->
+      l' = l.
+  Proof.
+    induction l; intros.
+    - inversion_ H.
+      discriminate.
+    - inversion_ H.
+      + discriminate.
+      + simpl in H0.
+        inversion_ H0.
+        specialize (IHl l0 H1).
+        subst.
+        reflexivity.
+  Qed.
+
+  Lemma list_generator_ensemble : forall (l : list TE) P Q,
+      -{{P}} eq l {{Q}} ->
+      -{{P}} UnfoldsTo l {{Q}}.
+  Proof.
+    intros. intros t Ht. unfold_ht.
+    apply unfold_list_generator in Ht. subst.
+    eapply (H l); eauto.
+  Qed.
+
+  Section parallel.
+    Context {G1 G2} `{Generator G1} `{Generator G2}.
+
+    Inductive ParallelGen :=
+    | gen_parallel : G1 -> G2 -> ParallelGen.
+
+    Inductive ParallelGenerator (g1 : G1) (g2 : G2) : option (TE * ParallelGen) -> Prop :=
+    | gen_par_nil :
+        (next g1) None ->
+        (next g2) None ->
+        ParallelGenerator g1 g2 None
+    | gen_par_l : forall te g1',
+        (next g1) (Some (te, g1')) ->
+        ParallelGenerator g1 g2 (Some (te, gen_parallel g1' g2))
+    | gen_par_r : forall te g2',
+        (next g2) (Some (te, g2')) ->
+        ParallelGenerator g1 g2 (Some (te, gen_parallel g1 g2')).
+
+    Global Instance parallelGenerator : Generator ParallelGen :=
+      {| next gen :=
+           match gen with
+           | gen_parallel g1 g2 => ParallelGenerator g1 g2
+           end
+      |}.
+  End parallel.
+End defn.
